sets are a partial order

Lean4_filters/set.lean
@@ -1,18 +1,31 @@
-def Set {α : Type} := α → Prop
-
 class HasMem (α : outParam $ Type u) (β : Type v) where
     mem : α → β → Prop
 
 infix:50 " ∈ " => HasMem.mem
 
-class HasLe (α : Type u) where
-    le : α → α → Prop
+def Set (α : Type u) := α → Prop
 
-infix:50 " ≤ " => HasLe.le
+namespace Set
 
+variable {α : Type u}
 
+instance : HasMem α (Set α) := ⟨λ a s => s a⟩
 
+theorem ext {s t : Set α} (h : ∀ x, x ∈ s ↔ x ∈ t) : s = t :=
+  funext $ λ x=> propext $ h x
+
+instance : HasLessEq (Set α) := ⟨λ s t => ∀ {x : α}, x ∈ s → x ∈ t⟩
   
+class PartialOrder (β : Type u) extends HasLessEq β where
+  refl (s : β) : s ≤ s
+  antisymm (s t : β) : s ≤ t → t ≤ s → s = t
+  trans (s t u : β) : s ≤ t → t ≤ u → s ≤ u
 
+instance : PartialOrder (Set α) where
+  refl := λ s x => id 
+  antisymm := λ s t hst hts => ext $ λ x => ⟨hst, hts⟩
+  trans := λ s t u hst htu x hxs => htu $ hst hxs
+
+end Set
 
 
